some progress on functor approach

secure_api/box/functor_box/Box.AE.fst
@@ -17,12 +17,16 @@ open Crypto.Symmetric.Bytes
 open Box.Flags
 open Box.Plain
 open Box.Indexing
+open Box.Key
 
 module MR = FStar.Monotonic.RRef
 module HH = FStar.HyperHeap
 module HS = FStar.HyperStack
 module MM = MonotoneMap
 module SPEC = Spec.SecretBox
+module Plain = Box.Plain
+module Key = Box.Key
+module ID = Box.Indexing
 
 
 let noncesize = SPEC.noncelen
@@ -36,21 +40,15 @@ val create_zero_bytes: n:nat -> Tot (b:bytes{Seq.length b = n})
 let create_zero_bytes n =
   Seq.create n (UInt8.uint_to_t 0)
 
-type ae_log_region (im:index_module) =
-  r:MR.rid{disjoint r (get_rgn im)}
-
-type ae_log_key (im:index_module) = (nonce*(i:id im))
-type ae_log_value (im:index_module) (pm:plain_module) (i:id im) = (cipher*protected_plain_t im (get_plain pm) i)
-let ae_log_range (im:index_module) (pm:plain_module) = fun (k:ae_log_key im) -> (ae_log_value im pm (snd k))
-let ae_log_inv (im:index_module) (pm:plain_module) (f:MM.map' (ae_log_key im) (ae_log_range im pm)) = True
-
-type ae_log (im:index_module) (rgn:ae_log_region im) (pm:plain_module) =
-  MM.t rgn (ae_log_key im) (ae_log_range im pm) (ae_log_inv im pm)
+type log_region (im:index_module) =
+  r:MR.rid{disjoint r (ID.get_rgn im)}
 
 (**
    The unprotected plaintext type.
 *)
 type ae_plain = b:bytes{Seq.length b / Spec.Salsa20.blocklen < pow2 32}
+
+type ae_protected_plain (im:index_module) (pm:plain_module) (i:id im) = m:Plain.protected_plain_t im (get_plain pm) i
 
 (**
   A helper function to obtain the length of a protected plaintext.
@@ -65,68 +63,108 @@ let length (b:bytes) = Seq.length b
    The key type is abstract and can only be accessed via the leak and coerce_key functions. This means that the adversary has no means
    of accessing the raw representation of any honest AE key if AE is idealized.
 *)
-noeq abstract type key (im:index_module) (pm:plain_module) =
-  | Key: i:id im -> rgn:ae_log_region im -> log:ae_log im rgn pm -> raw:aes_key -> key im pm
+abstract type key (im:index_module) = Key.key_t2 im
+//  | Key: i:id im -> rgn:log_region im -> log:message_log im rgn pm -> raw:aes_key -> key im pm
 
+
+val get_index: #im:index_module -> k:key im -> i:id im
+let get_index #im k =
+  k.i
+
+(**
+  Similar to the leak_key function, get_keyGT provides access to the raw representation of an AE key.
+  However, note that the GTot effect only allows use in type refinements and is erased upon extraction.
+*)
+val get_keyGT: #im:index_module -> k:key im -> GTot (raw_k:aes_key)
+let get_keyGT #im k =
+  k.raw
+
+type key_log_key (im:index_module) = i:id im
+type key_log_value (im:index_module) = (key im)
+let key_log_range (im:index_module) = fun (k:key_log_key im) -> (v:key_log_value im{v.i = k})
+let key_log_inv (im:index_module) (f:MM.map' (key_log_key im) (key_log_range im)) = True
+
+type key_log_t (im:index_module) (rgn:log_region im) = MM.t rgn (key_log_key im) (key_log_range im) (key_log_inv im)
+
+
+type message_log_key (im:index_module) = (nonce*(i:id im))
+type message_log_value (im:index_module) (pm:plain_module) (i:id im) = (cipher*protected_plain_t im (get_plain pm) i)
+let message_log_range (im:index_module) (pm:plain_module) = fun (k:message_log_key im) -> (message_log_value im pm (snd k))
+let message_log_inv (im:index_module) (pm:plain_module) (f:MM.map' (message_log_key im) (message_log_range im pm)) = True
+
+type message_log (im:index_module) (rgn:log_region im) (pm:plain_module) =
+  MM.t rgn (message_log_key im) (message_log_range im pm) (message_log_inv im pm)
+
+abstract noeq type ae_module (im:index_module) (pm:plain_module) =
+  | AM :
+    key_log_region: log_region im ->
+    message_log_region: (rgn:log_region im{disjoint rgn key_log_region}) ->
+    key_log: (key_log_t im key_log_region) ->
+    message_log: (message_log im message_log_region pm) ->
+    ae_module im pm
+
+let create im pm (klr:log_region im) message_log_region key_log =
+  AM klr message_log_region key_log
+
+
+val nonce_is_fresh: #im:index_module -> #pm:plain_module -> am:ae_module im pm -> i:id im -> n:nonce -> h:mem -> t:Type0{t <==> MM.fresh am.message_log (n,i) h}
+let nonce_is_fresh #im #pm am i n h =
+  MM.fresh am.message_log (n,i) h
+
+//val log_freshness_invariant: #im:index_module -> #pm:plain_module -> am:ae_module im pm -> h:mem -> Type0
+let log_freshness_invariant (#im:index_module) (#pm:plain_module) (am:ae_module im pm) (h:mem) =
+  MR.m_contains (get_log im) h
+  /\ MR.m_contains am.message_log h
+  /\ (forall i n . ID.fresh im (ID i) h ==> MM.fresh am.message_log (n,i) h)
+
+
+// Remove this later
+
+//assume val random_bytes: len:u32 -> ST (lbytes (UInt32.v len))
+//  (requires (fun h -> True))
+//  (ensures  (fun h0 _ h1 -> h0==h1))
 (**
    This function generates a fresh random key. Honest, as well as dishonest ids can be created using keygen. However, note that the adversary can
    only access the raw representation of dishonest keys. The log is created in a fresh region below the ae_key_region.
 *)
-#set-options "--z3rlimit 300 --max_ifuel 0 --max_fuel 0"
-val gen: #im:index_module -> #pm:plain_module -> i:id im -> rgn:ae_log_region im -> ST (k:key im pm{k.i=i})
+#set-options "--z3rlimit 2000 --max_ifuel 1 --max_fuel 0"
+val gen: im:index_module -> pm:plain_module -> am:ae_module im pm -> i:id im -> ST (k:key im{get_index k=i})
   (requires (fun h0 ->
-    fresh im (ID i) h0 \/ honest im (ID i)
+    (fresh im (ID i) h0 \/ honest im (ID i))
+    /\ log_freshness_invariant #im #pm am h0
+    ///\ (forall (i:id im) (n:nonce) . ID.fresh im (ID i) h0 ==> MM.fresh am.message_log (n,i) h0)
   ))
   (ensures  (fun h0 k h1 ->
-    let modified_regions = (Set.singleton rgn) in
-    modifies modified_regions h0 h1
+    modifies Set.empty h0 h1
+    /\ log_freshness_invariant #im #pm am h1
+    ///\ (forall (i:id im) (n:nonce) . ID.fresh im (ID i) h1 ==> MM.fresh am.message_log (n,i) h1)
   ))
-let gen #im #pm i rgn =
-  let rnd_k = random_bytes (UInt32.uint_to_t keysize) in
-  let key_region = new_region rgn in
-  let key_log = MM.alloc #key_region #(ae_log_key im) #(ae_log_range im pm) #(ae_log_inv im pm) in
-  Key i key_region key_log rnd_k
 
+let gen im pm am i =
+  match MM.lookup am.key_log i with
+  | Some k -> k
+  | None ->
+    let rnd_k = random_bytes (UInt32.uint_to_t keysize) in
+    let k:key im = Key i rnd_k in
+    recall_log im;
+    MR.m_recall am.message_log;
+    k
 
 (**
    The coerce function transforms a raw aes_key into an abstract key. Only dishonest ids can be used
    with this function.
 *)
 #set-options "--z3rlimit 500 --max_ifuel 1 --max_fuel 1"
-val coerce: #im:index_module -> #pm:plain_module -> i:id im -> rgn:ae_log_region im -> raw_k:aes_key -> ST (k:key im pm{k.i=i /\ k.raw = raw_k})
-  (requires (fun h0 ->
-    dishonest im (ID i)
-    \/ fresh im (ID i) h0
-  ))
-  (ensures  (fun h0 k h1 ->
-    let modified_regions = Set.union (Set.singleton (get_rgn im)) (Set.singleton rgn) in
-    let (i1,i2) = i in
-    ((~(fresh im (SUBID i1) h0) /\ ~(fresh im (SUBID i2) h0)) ==> modifies (Set.singleton rgn) h0 h1)
-    /\ (fresh im (SUBID i1) h0 /\ ~(fresh im (SUBID i2) h0) ==> MR.m_sel h1 (get_log im) == MM.upd (MR.m_sel h0 (get_log im)) i1 false /\ modifies modified_regions h0 h1)
-    /\ (fresh im (SUBID i2) h0 /\ ~(fresh im (SUBID i1) h0) ==> MR.m_sel h1 (get_log im) == MM.upd (MR.m_sel h0 (get_log im)) i2 false /\ modifies modified_regions h0 h1)
-    /\ (fresh im (SUBID i1) h0 /\ fresh im (SUBID i2) h0 ==> MR.m_sel h1 (get_log im) == MM.upd (MM.upd (MR.m_sel h0 (get_log im)) i1 false) i2 false /\ modifies modified_regions h0 h1)
-  ))
-let coerce #im #pm i rgn raw_k =
-  recall_log im;
-  make_dishonest im (ID i);
-  let key_region = new_region rgn in
-  let key_log = MM.alloc #key_region #(ae_log_key im) #(ae_log_range im pm) #(ae_log_inv im pm) in
-  Key i key_region key_log raw_k
+val coerce: #im:index_module -> #pm:plain_module -> am:ae_module im pm -> i:id im -> raw_k:aes_key -> (k:key im{get_index k=i /\ get_keyGT k = raw_k})
+let coerce #im #pm am i raw_k =
+  Key i raw_k
 
 (**
    The leak_key function transforms an abstract key into a raw aes_key.
    The refinement type on the key makes sure that no honest keys can be leaked.
 *)
-val leak: #im:index_module -> #pm:plain_module -> k:key im pm{(dishonest im (ID k.i)) \/ ~(b2t ae_ind_cca)} -> Tot (raw_k:aes_key{raw_k=k.raw})
+val leak: #im:index_module -> #pm:plain_module -> k:key im{(dishonest im (ID (get_index k))) \/ ~(b2t ae_ind_cca)} -> Tot (raw_k:aes_key{raw_k=get_keyGT k})
 let leak #im #pm k =
-  k.raw
-
-(**
-   Similar to the leak_key function, get_keyGT provides access to the raw representation of an AE key.
-   However, note that the GTot effect only allows use in type refinements and is erased upon extraction.
-*)
-val get_keyGT: #im:index_module -> #pm:plain_module -> k:key im pm -> GTot (raw_k:aes_key{raw_k=k.raw})
-let get_keyGT #im #pm k =
   k.raw
 
 //////////////////////////////////////////////////////////////////////////////////////////////////////////////
@@ -138,43 +176,46 @@ let get_keyGT #im #pm k =
 (**
    Encrypt a a message under a key. Idealize if the key is honest and ae_ind_cca true.
 *)
-val encrypt: #im:index_module -> #pm:plain_module{get_plain pm == ae_plain} -> #(i:id im) -> n:nonce -> k:key im pm{k.i=i} -> (m:Plain.protected_plain_t im (get_plain pm) i{Plain.length #im #pm #i m / Spec.Salsa20.blocklen < pow2 32}) -> ST cipher
+val encrypt: #im:index_module -> #pm:plain_module{get_plain pm == ae_plain} -> am:ae_module im pm -> #(i:id im) -> n:nonce -> k:key im{get_index k=i} -> m:ae_protected_plain im pm i{Plain.length #im #pm #i m / Spec.Salsa20.blocklen < pow2 32} -> ST cipher
   (requires (fun h0 ->
     (fresh im (ID i) h0 \/ registered im (ID i)) // No in-between states of keys (i.e.) where one of the shares is fresh and one is registerd
     /\ ((honest im (ID i)) ==>
-               (MR.m_contains k.log h0
-               /\ MM.fresh k.log (n,i) h0)) // Nonce freshness
-    /\ (fresh im (ID i) h0 ==>
-             (m_sel h0 k.log == MM.empty_map (ae_log_key im) (ae_log_range im pm))) // If the key is fresh, so has to be its log.
+               (MR.m_contains am.message_log h0
+               /\ MM.fresh am.message_log (n,i) h0)) // Nonce freshness
+    ///\ (fresh im (ID i) h0 ==>
+    //         (m_sel h0 am.message_log == MM.empty_map (message_log_key im) (message_log_range im pm))) // If the key is fresh, so has to be its log.
+    /\ log_freshness_invariant #im #pm am h0
   ))
   (ensures  (fun h0 c h1 ->
-    let modified_regions_fresh = Set.union (Set.singleton k.rgn) (Set.singleton (get_rgn im)) in
-    let modified_regions_honest = Set.singleton k.rgn in
+    let modified_regions_fresh = Set.union (Set.singleton am.message_log_region) (Set.singleton (ID.get_rgn im)) in
+    let modified_regions_honest = Set.singleton am.message_log_region in
     registered im (ID i)
     /\ (fresh im (ID i) h0 ==>
                        (let (i1,i2) = i in
                        honest im (ID i)
-                       /\ MR.m_contains (get_log im) h1
-                       /\ (MR.m_sel h1 (get_log im) == MM.upd (MM.upd (MR.m_sel h0 (get_log im)) i1 true) i2 true /\ modifies modified_regions_fresh h0 h1)))
+                       /\ MR.m_contains (ID.get_log im) h1
+                       /\ (MR.m_sel h1 (ID.get_log im) == MM.upd (MM.upd (MR.m_sel h0 (ID.get_log im)) i1 true) i2 true /\ modifies modified_regions_fresh h0 h1)))
     /\ ((~(fresh im (ID i) h0) /\ honest im (ID i)) ==> HS.modifies modified_regions_honest h0 h1)
     /\ (dishonest im (ID i) ==> h0 == h1)
     /\ ((honest im (ID i) /\ b2t ae_ind_cpa)
-        ==> (c = SPEC.secretbox_easy (create_zero_bytes (Plain.length #im #pm #i m)) k.raw n))
+        ==> (c = SPEC.secretbox_easy (create_zero_bytes (Plain.length #im #pm #i m)) (get_keyGT k) n))
     /\ ((dishonest im (ID i) \/ ~(b2t ae_ind_cpa))
-        ==> (eq2 #cipher c (SPEC.secretbox_easy (Plain.repr #im #pm #i m) k.raw n)))
+        ==> (eq2 #cipher c (SPEC.secretbox_easy (Plain.repr #im #pm #i m) (get_keyGT k) n)))
     /\ ((honest im (ID i)) ==>
-                      (MR.m_contains k.log h1
-                      /\ MR.witnessed (MM.contains k.log (n,i) (c,m))
-                      /\ MR.m_sel h1 k.log == MM.upd (MR.m_sel h0 k.log) (n,i) (c,m)))
+                      (MR.m_contains am.message_log h1
+                      /\ MR.witnessed (MM.contains am.message_log (n,i) (c,m))
+                      /\ MR.m_sel h1 am.message_log == MM.upd (MR.m_sel h0 am.message_log) (n,i) (c,m)))
+    /\ log_freshness_invariant #im #pm am h1
   ))
 
-#set-options "--z3rlimit 400 --max_ifuel 1 --max_fuel 0"
-let encrypt #im #pm #i n k m =
-  MR.m_recall k.log;
+#set-options "--z3rlimit 900 --max_ifuel 1 --max_fuel 0"
+let encrypt #im #pm am #i n k m =
+  MR.m_recall am.message_log;
   recall_log im;
   if is_fresh im (ID i) then (
     make_honest im (ID i)
   );
+  let h0 = get() in
   recall_log im;
   lemma_honest_or_dishonest im (ID i);
   let h = get_reg_honesty im (ID i) in
@@ -192,9 +233,11 @@ let encrypt #im #pm #i n k m =
   in
   let  c = SPEC.secretbox_easy p k.raw n in
   if HONEST? h then (
-    MR.m_recall k.log;
+    let h1 = get() in
+    assert(h0==h1);
+    MR.m_recall am.message_log;
     recall_log im;
-    MM.extend k.log (n,i) (c,m)
+    MM.extend am.message_log (n,i) (c,m)
     );
   c
 
@@ -203,41 +246,41 @@ let encrypt #im #pm #i n k m =
    Decrypt a ciphertext c using a key k. If the key is honest and ae_int_ctxt is idealized,
    try to obtain the ciphertext from the log. Else decrypt via concrete implementation.
 *)
-
-val decrypt: #im:index_module -> #pm:plain_module{get_plain pm == ae_plain} -> #(i:id im) -> n:nonce -> k:key im pm{k.i=i} -> c:cipher -> ST (option (m:Plain.protected_plain_t im (get_plain pm) i))
+val decrypt: #im:index_module -> #pm:plain_module{get_plain pm == ae_plain} -> am:ae_module im pm -> #(i:id im) -> n:nonce -> k:key im{get_index k=i} -> c:cipher -> ST (option (ae_protected_plain im pm i))
   (requires (fun h0 ->
     (fresh im (ID i) h0 \/ registered im (ID i)) // No in-between states of keys (i.e.) where one of the shares is fresh and one is registerd
-    /\ (fresh im (ID i) h0 ==>
-             (m_sel h0 k.log == MM.empty_map (ae_log_key im) (ae_log_range im pm))) // If the key is fresh, so has to be its log.
+    /\ log_freshness_invariant #im #pm am h0
   ))
   (ensures  (fun h0 p h1 ->
-    let modified_regions_fresh = Set.union (Set.singleton k.rgn) (Set.singleton (get_rgn im)) in
-    let modified_regions_honest = Set.singleton k.rgn in
+    let modified_regions_fresh = Set.union (Set.singleton am.message_log_region) (Set.singleton (ID.get_rgn im)) in
+    let modified_regions_honest = Set.singleton am.message_log_region in
     registered im (ID i)
     /\ (fresh im (ID i) h0 ==>
                 (let (i1,i2) = i in
                 honest im (ID i)
-                /\ MR.m_contains (get_log im) h1
-                /\ (MR.m_sel h1 (get_log im) == MM.upd (MM.upd (MR.m_sel h0 (get_log im)) i1 true) i2 true /\ modifies modified_regions_fresh h0 h1)))
+                /\ MR.m_contains (ID.get_log im) h1
+                /\ (MR.m_sel h1 (ID.get_log im) == MM.upd (MM.upd (MR.m_sel h0 (ID.get_log im)) i1 true) i2 true /\ modifies modified_regions_fresh h0 h1)))
     /\ (((honest im (ID i) \/ dishonest im (ID i)) /\ ~(fresh im (ID i) h0) ) ==> h0 == h1)
     /\ ((~(b2t ae_int_ctxt) \/ dishonest im (ID i))
-      ==> ((Some? (SPEC.secretbox_open_easy c k.raw n)
-        ==> Some? p /\ Some?.v p == Plain.coerce #im #pm #i (Some?.v (SPEC.secretbox_open_easy c k.raw n)))
-  /\ ((None? (SPEC.secretbox_open_easy c k.raw n))
+      ==> ((Some? (SPEC.secretbox_open_easy c (get_keyGT k) n)
+        ==> Some? p /\ Some?.v p == Plain.coerce #im #pm #i (Some?.v (SPEC.secretbox_open_easy c (get_keyGT k) n)))
+  /\ ((None? (SPEC.secretbox_open_easy c (get_keyGT k) n))
     ==> None? p)
       ))
     /\ ((b2t ae_int_ctxt /\ honest im (ID i))
         ==> (Some? p
-          ==> (MM.defined k.log (n,i) h0 /\ (fst (MM.value k.log (n,i) h0) == c )
-            /\ Some?.v p == snd (MM.value k.log (n,i) h0)))
+          ==> (MM.defined am.message_log (n,i) h0 /\ (fst (MM.value am.message_log (n,i) h0) == c )
+            /\ Some?.v p == snd (MM.value am.message_log (n,i) h0)))
     /\ (None? p
-    ==> (MM.fresh k.log (n,i) h0 \/ c =!= fst (MM.value k.log (n,i) h0)))
+    ==> (MM.fresh am.message_log (n,i) h0 \/ c =!= fst (MM.value am.message_log (n,i) h0)))
    )
+   /\ log_freshness_invariant #im #pm am h1
   ))
 
 
-let decrypt #im #pm #i n k c =
-  MR.m_recall k.log;
+#set-options "--z3rlimit 1900 --max_ifuel 1 --max_fuel 0"
+let decrypt #im #pm am #i n k c =
+  MR.m_recall am.message_log;
   recall_log im;
   if is_fresh im (ID i) then (
     make_honest im (ID i)
@@ -251,8 +294,10 @@ let decrypt #im #pm #i n k c =
     | DISHONEST ->
       false
   in
+  MR.m_recall am.message_log;
+  recall_log im;
   if ideal then
-    match MM.lookup k.log (n,i) with
+    match MM.lookup am.message_log (n,i) with
     | Some (c',m') ->
       if c' = c then
         Some m'
@@ -262,5 +307,6 @@ let decrypt #im #pm #i n k c =
   else
     let p = (SPEC.secretbox_open_easy c k.raw n) in
     match p with
-    | Some p' -> Some (Plain.coerce #im #pm #i p')
+    | Some p' ->
+      Some (Plain.coerce #im #pm #i p')
     | None -> None
